Labs/Lab_6/Ex_1.dfy
@@ -1,0 +1,89 @@
+
+//specification should not leak implementation details 
+
+class   PVNode   {
+    var   data   :   int
+    var   pri   :   int
+    var   next   :   PVNode?
+    ghost   var   pvlist   :   seq <( int , int ) >
+    ghost   var   footprint   :   set < PVNode >
+
+    ghost function Valid() : bool
+       reads this, footprint
+    {
+    if next == null
+    then this.pvlist == [(data, pri)] && this.footprint == {this}
+    else 
+    next in footprint
+    && pvlist == [(data, pri)] + next.pvlist
+    && footprint == {this} + next.footprint
+    && this !in next.footprint
+    && sortedPVList(pvlist)
+    && next.Valid()
+    
+
+    }
+
+    constructor (p : int, v : int)
+    ensures Valid()
+        && footprint == {this}
+        && pvlist == [(v,p)]
+    {
+        this.pri := p;
+        this.data:= v;
+        this.next:= null;
+        this.pvlist := [(v,p)];
+        this.footprint := {this};
+    }
+
+    method insertPVPair ( p :   int , v : int ) returns (r:PVNode )
+    requires Valid () && p>=0
+    ensures Valid () && r.Valid()
+    ensures r.pvlist[0].1 <= max(p, old(this.pvlist[0].1))
+    ensures fresh(r.footprint - old(this.footprint))
+
+
+    modifies footprint
+    decreases footprint
+    {
+        if(p <= this.pri){
+            r:=new PVNode(p,v);
+            r.next:= this;
+            r.pvlist:= [(v,p)] + this.pvlist;
+            r.footprint:={r} + this.footprint;
+            return;
+        }else{
+            r:=this;
+            if(this.next == null){
+                var aux := new PVNode(p,v);
+                this.next:=aux;
+                this.pvlist:=[(this.data, this.pri), (v,p)];
+                this.footprint:={this, aux};
+                return;
+            }else{
+                assert this.pri == this.pvlist[0].1;
+                assert next.pri == this.pvlist[1].1;
+                var aux := this.next.insertPVPair(p,v);
+                this.next:=aux;
+                this.pvlist:=[(this.data, this.pri)] + aux.pvlist;
+                this.footprint:={this} + aux.footprint;
+                return;
+            }
+        }
+    }
+
+}
+
+function sortedPVList(pvlist: seq<(int, int)>):bool{
+    forall i,j :: 0<=i<=j<|pvlist| ==> pvlist[i].1 <= pvlist[j].1
+}
+
+function max(x:int, y:int):int{
+    if x <= y
+    then y
+    else x
+}
+
+
+
+
